transformations/Moore2Mealy/Moore2Mealy.v
@@ -46,8 +46,25 @@ Definition Moore2Mealy' :=
                           t.(Moore.Transition_id)
                           t.(Moore.Transition_input)
                           (value (option_map Moore.State_output (Moore.getTransition_target m t))) >> 
+
           <<<
-             LINK  
+         (*    LINK  
+              Mealy.Transition_source_K //
+              (fun tls _ m moore_tr mealy_tr =>
+                 match Moore.getTransition_source m moore_tr with
+                 | Some s =>
+                     match Resolve.resolve tls "s" 
+                             ( (Moore.StateElement s) :: nil)
+                     with 
+                     | Some (StateElement s') =>
+                            Some (Glue.Build_Glue _ _ mealy_tr s')   
+                     | _ => None 
+                     end
+                       
+                 | None => None
+                 end) ; *)
+
+        LINK  
               Mealy.Transition_source_K //
               (fun tls _ m moore_tr mealy_tr =>
                 maybeBuildTransitionSource mealy_tr
