transformations/Moore2Mealy/theorems/WFStable.v
@@ -14,3 +14,29 @@ Lemma unique_ids_preserved_fw : forall m,
 Proof.
   intros ; apply MealyWF.always_unique_ids.
 Qed.
+
+Import Model Semantics.
+
+Lemma WF_sourceLink_left_stable :
+  forall m,
+    Moore.WF_target m ->
+    Moore.WF_source m -> 
+    MooreWF.WF_sourceLink_left m -> 
+    MealyWF.WF_sourceLink_left (Semantics.execute Moore2Mealy.Moore2Mealy m).
+Proof.
+  intros m WF1 WF2 WF4.
+  unfold MealyWF.WF_sourceLink_left.
+  intros. 
+
+  destruct lk1 as (t' & s').
+  destruct lk2 as (t'' & s'').
+  simpl in H1. subst t''.
+  f_equal.
+  
+  destruct (Links.source_link_bw _ WF1 WF2 _ _ H) as (s1 & C1 & IN1).
+  destruct (Links.source_link_bw _ WF1 WF2 _ _ H0) as (s2 & C2 & IN2).
+
+  specialize (WF4 _ _ IN1 IN2 (eq_refl _)). 
+  PropUtils.inj WF4.
+  reflexivity.
+Qed.
